concurrency/juicy/Clight_safety.v
@@ -69,7 +69,7 @@ Definition initial_Clight_state : Clight.state :=
              (map (fun x => Clight.Etempvar (fst x) (snd x))
              (Clight_new.params_of_types 2 (Clight_new.params_of_fundef f))))
              (Clight.Kseq (Clight.Sloop Clight.Sskip Clight.Sskip) Clight.Kstop) Clight.empty_env
-             (Clight_new.temp_bindings 1 [Vptr (projT1 (spr CPROOF)) Ptrofs.zero]) init_mem.
+             (temp_bindings 1 [Vptr (projT1 (spr CPROOF)) Ptrofs.zero]) init_mem.
 
 (*...And we should be able to construct an initial state from the Clight_new and mem.*)
 (* See also veric/Clight_sim.v. *)
@@ -510,7 +510,8 @@ Proof.
     inv Hstep.
     inv H; simpl.
     apply memsem_lemmas.mem_step_obeys_cur_write; auto.
-    apply memsem_lemmas.mem_step_refl.
+  (* apply memsem_lemmas.mem_step_refl. *)
+    eapply mem_step_alloc; eauto.
   - intros.
     inv H.
     inv H0; simpl.
